rework kraken to simplify primitives
Simplify primitives to just send and recv.

Implement said primitives in OCaml.

Tweak Kernel to reduce axioms.

kernel-template/ml/primitives/KrakenBaseImpl.ml
@@ -1,115 +1,102 @@
+let (|>) x f =
+  f x
+
 (*
- * UTILITIES
+ * ML <-> Coq
+ *)
+
+let bits_of_ascii = function
+  | MlCoq.Ascii (a1, a2, a3, a4, a5, a6, a7, a8) ->
+      [a8; a7; a6; a5; a4; a3; a2; a1]
+
+let ascii_of_bits = function
+  | [a8; a7; a6; a5; a4; a3; a2; a1] ->
+      MlCoq.Ascii (a1, a2, a3, a4, a5, a6, a7, a8)
+  | _ ->
+      failwith "ascii_of_bits"
+
+let char_of_bits b =
+  b |> List.map (function true -> 1 | false -> 0)
+    |> List.fold_left (fun n b -> 2 * n + b) 0
+    |> Char.chr
+
+let bits_of_char c =
+  let rec last_bits i acc n =
+    if i = 0 then
+      acc
+    else
+      last_bits (i - 1) (n land 1 :: acc) (n lsr 1)
+  in
+  c |> Char.code
+    |> last_bits 8 []
+    |> List.map (function 0 -> false | _ -> true)
+
+let char_of_ascii a =
+  a |> bits_of_ascii
+    |> char_of_bits
+
+let ascii_of_char c =
+  c |> bits_of_char
+    |> ascii_of_bits
+
+let explode s =
+  let rec loop i l =
+    if i < 0 then l
+    else loop (i - 1) (s.[i] :: l)
+  in
+  loop (String.length s - 1) []
+
+let implode cs =
+  let s = String.make (List.length cs) (Char.chr 0) in
+  let rec loop i = function
+    | c::cs' ->
+        s.[i] <- c;
+        loop (i + 1) cs'
+    | [] -> s
+  in
+  loop 0 cs
+
+let string_of_str s =
+  s |> List.map char_of_ascii
+    |> implode
+
+let str_of_string s =
+  s |> explode
+    |> List.map ascii_of_char
+
+let int_of_num n =
+  Char.code (char_of_ascii n)
+
+(*
+ * PRIMITIVES
  *)
 
 let mkstr =
   Printf.sprintf
 
-let null =
-  Char.chr 0
-
-let mkbuf n =
-  String.make n null
-
-(* explode : string -> char list *)
-let explode s =
-  let rec loop i l =
-    if i < 0 then
-      l
-    else
-      loop (i - 1) (s.[i] :: l)
-  in
-  loop (String.length s - 1) []
-
-(* implode : char list -> string *)
-let implode cs =
-  let s = mkbuf (List.length cs) in
-  let rec loop i = function
-    | c::cs' -> begin
-        s.[i] <- c;
-        loop (i + 1) cs'
-    end
-    | [] ->
-        s
-  in
-  loop 0 cs
-
-(* decode bytes of str to a num *)
-let str_num s =
-  List.fold_left (fun acc c -> acc * 256 + Char.code c) 0 (explode s)
-
-(* encode bytes of num to a str *)
-let num_str n =
-  let rec loop acc n =
-    if n < 256 then
-      Char.chr n :: acc
-    else
-      loop (Char.chr (n mod 256) :: acc) (n / 256)
-  in
-  if n < 0 then
-    failwith (mkstr "ERROR: num_str got negative arg %d" n)
-  else
-    implode (List.rev (loop [] n))
-
-(* prepend fill to s until it reaches len *)
-let rec pad_front fill len s =
-  if String.length s < len then
-    pad_front fill len (Char.escaped fill ^ s)
-  else
-    s
-
-(*
- * LOGGING
- *)
-
 let log msg =
   ()
 
-(*
- * IO OPERATIONS
- *)
+type chan =
+  Unix.file_descr
 
-(* dummy args represent trace *)
-
-type chan = Unix.file_descr
-
-let recvN c  _ =
-  let b = mkbuf 4 in
-  let n = Unix.read c b 0 4 in
-  if n <> 4 then
-    failwith (mkstr "ERROR: recvN only read %d bytes instead of 4" n)
+let recv c n _ =
+  let n = int_of_num n in
+  let s = String.make n (Char.chr 0) in
+  let r = Unix.read c s 0 n in
+  if r <> n then
+    failwith (mkstr "recv expected %d but got %d" n r)
   else begin
-    let x = str_num b in
-    log (mkstr "recvN got '%s' which decoded to %d" b x);
-    x
+    log (mkstr "recv '%s'" (String.escaped s));
+    str_of_string s
   end
 
-let recvS c bsize _ =
-  let b = mkbuf bsize in
-  let n = Unix.read c b 0 bsize in
-  if n <> bsize then
-    failwith (mkstr "ERROR: recvS only read %d bytes insted of %d" n bsize)
+let send c s _ =
+  let s = string_of_str s in
+  let n = String.length s in
+  let w = Unix.write c s 0 n in
+  if w <> n then
+    failwith (mkstr "send expected %d but put %d" n w)
   else begin
-    log (mkstr "recvS got '%s'" b);
-    b
+    log (mkstr "send '%s'" (String.escaped s))
   end
-
-let sendN c n _ =
-  let b = pad_front null 4 (num_str n) in
-  if String.length b <> 4 then
-    failwith (mkstr "ERROR: sendN got oversized arg %d" n)
-  else begin
-    let n = Unix.write c b 0 4 in
-    if n <> 4 then
-      failwith (mkstr "ERROR: sendN only wrote %d bytes instead of 4" n)
-    else
-      log (mkstr "sendN put %d which encoded to '%s'" n (String.escaped b))
-  end
-
-let sendS c b _ =
-  let bsize = String.length b in
-  let n = Unix.write c b 0 bsize in
-  if n <> bsize then
-    failwith (mkstr "ERROR: sendS tried to put '%s' but only wrote %d bytes insted of %d" b n bsize)
-  else
-    log (mkstr "sendS put '%s'" b)
