src/common.ml
@@ -32,6 +32,29 @@ let explode s =
   in
   loop (String.length s - 1) []
 
+let bits n =
+  let rec loop i acc n =
+    if i = 0 then
+      acc
+    else if n land 1 = 0 then
+      loop (i - 1) (false :: acc) (n lsr 1)
+    else
+      loop (i - 1) (true :: acc) (n lsr 1)
+  in
+  loop 32 [] n
+
+let rec take n l =
+  match n, l with
+  | 0, _ -> []
+  | _, [] -> failwith "take"
+  | n, x :: xs -> x :: take (n - 1) xs
+
+let rec drop n l =
+  match n, l with
+  | 0, l -> l
+  | _, [] -> failwith "drop"
+  | n, x :: xs -> drop (n - 1) xs
+
 let readline f =
   try
     Some (input_line f)
