kernel-template/coq/KrakenBase.v
@@ -1,72 +1,48 @@
 Require Import List.
 Require Import Ascii.
-Require Import BinNat.
-Require Import Nnat.
 Require Import Ynot.
 
-Open Local Scope stsepi_scope.
 Open Local Scope hprop_scope.
-
-Definition num : Set :=
-  N.
+Open Local Scope stsepi_scope.
 
 Definition str : Set :=
   list ascii.
 
-Definition len (s: str) : N :=
-  N_of_nat (length s).
+Inductive num : Set :=
+| Num : ascii -> num.
+
+Definition nat_of_num (n: num) : nat :=
+  match n with
+    | Num a1 => nat_of_ascii a1
+  end.
 
 Axiom chan : Set.
 
 Inductive Action : Set :=
-| RecvN : chan -> N -> Action
-| RecvS : chan -> N -> str -> Action
-| SendN : chan -> N -> Action
-| SendS : chan -> str -> Action.
+| Recv : chan -> str -> Action
+| Send : chan -> str -> Action.
 
 Definition Trace : Set :=
   list Action.
 
-Definition RecvNum (c: chan) (n: num) : Trace :=
-  RecvN c n ::
-  nil.
-
-Definition SendNum (c: chan) (n: num) : Trace :=
-  SendN c n ::
-  nil.
-
-Definition RecvStr (c: chan) (s: str) : Trace :=
-  RecvS c (len s) s ::
-  RecvN c (len s) ::
-  nil.
-
-Definition SendStr (c: chan) (s: str) : Trace :=
-  SendS c s ::
-  SendN c (len s) ::
-  nil.
-
-Axiom bound : chan -> hprop.
 Axiom traced : Trace -> hprop.
 
-Axiom recvN:
-  forall (c: chan) (tr: [Trace]),
-  STsep (tr ~~ traced tr * bound c)
-        (fun n => tr ~~ traced (RecvN c n :: tr) * bound c).
+Axiom bound : chan -> hprop.
 
-Axiom recvS:
-  forall (c: chan) (n: N) (tr: [Trace]),
+Axiom recv:
+  forall (c: chan) (n: num) (tr: [Trace]),
   STsep (tr ~~ traced tr * bound c)
-        (fun s => tr ~~ traced (RecvS c n s :: tr) * bound c * [n = len s]).
+        (fun (s: str) => tr ~~ traced (Recv c s :: tr) * bound c * [nat_of_num n = length s]).
 
-Axiom sendN:
-  forall (c: chan) (n: N) (tr: [Trace]),
-  STsep (tr ~~ traced tr * bound c)
-        (fun (_: unit) => tr ~~ traced (SendN c n :: tr) * bound c).
-
-Axiom sendS:
+Axiom send:
   forall (c: chan) (s: str) (tr: [Trace]),
   STsep (tr ~~ traced tr * bound c)
-        (fun (_: unit) => tr ~~ traced (SendS c s :: tr) * bound c).
+        (fun (_: unit) => tr ~~ traced (Send c s :: tr) * bound c).
+
+Definition RecvNum (c: chan) (n: num) : Trace :=
+  match n with
+    | Num a1 => Recv c (a1 :: nil) :: nil
+  end.
 
 Definition recvNum:
   forall (c: chan) (tr: [Trace]),
@@ -74,25 +50,43 @@ Definition recvNum:
         (fun n => tr ~~ traced (RecvNum c n ++ tr) * bound c).
 Proof.
   intros; refine (
-    n <- recvN c
+    s <- recv c (Num one)
       tr;
-    {{ Return n }}
+    match s with
+      | a1 :: nil =>
+        {{ Return (Num a1) }}
+      | _ => (* bogus *)
+        {{ Return (Num zero) }}
+    end
   );
-  sep fail auto.  
+  sep fail auto.
+  compute in H; discriminate.
+  compute in H; discriminate.
 Qed.
 
+Definition SendNum (c: chan) (n: num) : Trace :=
+  match n with
+    | Num a1 => Send c (a1 :: nil) :: nil
+  end.
+
 Definition sendNum:
-  forall (c: chan) (n: N) (tr: [Trace]),
+  forall (c: chan) (n: num) (tr: [Trace]),
   STsep (tr ~~ traced tr * bound c)
         (fun (_: unit) => tr ~~ traced (SendNum c n ++ tr) * bound c).
 Proof.
   intros; refine (
-    sendN c n
-      tr;;
-    {{ Return tt }}
+    match n with
+      | Num a1 =>
+        send c (a1 :: nil)
+          tr;;
+        {{ Return tt }}
+    end
   );
-  sep fail auto.  
+  sep fail auto.
 Qed.
+
+Definition RecvStr (c: chan) (s: str) : Trace :=
+  Recv c s :: RecvNum c (Num (ascii_of_nat (length s))).
 
 Definition recvStr:
   forall (c: chan) (tr: [Trace]),
@@ -100,14 +94,20 @@ Definition recvStr:
         (fun s => tr ~~ traced (RecvStr c s ++ tr) * bound c).
 Proof.
   intros; refine (
-    n <- recvN c
+    n <- recvNum c
       tr;
-    s <- recvS c n
-      (tr ~~~ RecvN c n :: tr);
+    s <- recv c n
+      (tr ~~~ RecvNum c n ++ tr);
     {{ Return s }}
   );
-  sep fail auto.  
+  sep fail auto.
+  destruct n; simpl in *.
+  rewrite <- H. rewrite ascii_nat_embedding.
+  sep fail auto.
 Qed.
+
+Definition SendStr (c: chan) (s: str) : Trace :=
+  Send c s :: SendNum c (Num (ascii_of_nat (length s))).
 
 Definition sendStr:
   forall (c: chan) (s: str) (tr: [Trace]),
@@ -115,10 +115,11 @@ Definition sendStr:
         (fun (_: unit) => tr ~~ traced (SendStr c s ++ tr) * bound c).
 Proof.
   intros; refine (
-    sendN c (len s)
+    let n := Num (ascii_of_nat (length s)) in
+    sendNum c n
       tr;;
-    sendS c s
-      (tr ~~~ SendN c (len s) :: tr);;
+    send c s
+      (tr ~~~ SendNum c n ++ tr);;
     {{ Return tt }}
   );
   sep fail auto.  
