kernel-template/coq/Extract.v
@@ -2,11 +2,9 @@ Require Import Ynot.Extract.
 Require Import KrakenBase.
 Require Import Kernel.
 
-Extract Constant KrakenBase.chan  => "KrakenBaseImpl.chan".
-Extract Constant KrakenBase.recvN => "KrakenBaseImpl.recvN".
-Extract Constant KrakenBase.recvS => "KrakenBaseImpl.recvS".
-Extract Constant KrakenBase.sendN => "KrakenBaseImpl.sendN".
-Extract Constant KrakenBase.sendS => "KrakenBaseImpl.sendS".
+Extract Constant KrakenBase.chan => "KrakenBaseImpl.chan".
+Extract Constant KrakenBase.recv => "KrakenBaseImpl.recv".
+Extract Constant KrakenBase.send => "KrakenBaseImpl.send".
 
 Cd "../ml".
 Recursive Extraction Library Kernel.
